canonical forms

test.lean
@@ -1,38 +1,20 @@
 import TextbookTemplate
 open TextbookTemplate
 
-inductive ty : Type :=
-  | Bool : ty
-  | Nat : ty
-
-inductive has_type : tm -> ty -> Prop where
-| t_true : has_type {{true}} .Bool
-| t_false : has_type {{false}} .Bool
-| t_ite :
-  ∀ g thn els : tm,
-  has_type g .Bool ->
-  has_type thn t ->
-  has_type els t ->
-  has_type {{if [g] then [thn] else [els]}} t
-| t_zro : has_type {{zero}} .Nat
-| t_succ :
-  ∀ t : tm,
-  has_type t .Nat ->
-  has_type {{succ [t]}} .Nat
-| t_pred :
-  ∀ t,
-  has_type t .Nat ->
-  has_type {{pred [t]}} .Nat
-| t_zero? :
-  ∀ t,
-  has_type t .Nat ->
-  has_type {{zero? [t]}} .Bool
-
 theorem bool_canonical :
-  ∀ t : tm, has_type t .Bool -> value t -> bvalue t := by
+  ∀ t,
+  has_type t .Bool -> value t -> bvalue t := by
   intro t ty v
-  cases ty with
-  | t_true => constructor
-  | t_false => constructor
-  | t_ite =>
-    sorry
+  cases v with
+  | inl => assumption
+  | inr =>
+    rename_i h
+    cases ty <;> contradiction
+
+theorem num_canonical :
+  ∀ t,
+  has_type t .Nat -> value t -> nvalue t := by
+  intro t ty v
+  cases v with
+  | inl => cases ty <;> contradiction
+  | inr => assumption
