TextbookTemplate.lean
@@ -266,3 +266,26 @@ inductive has_type : tm -> ty -> Prop where
   has_type t .Nat ->
   has_type {{zero? [t]}} .Bool
 ```
+
+Some useful metatheoretic properties of the
+type system:
+
+```savedLean
+theorem bool_canonical :
+  ∀ t,
+  has_type t .Bool -> value t -> bvalue t := by
+  intro t ty v
+  cases v with
+  | inl => assumption
+  | inr =>
+    rename_i h
+    cases ty <;> contradiction
+
+theorem num_canonical :
+  ∀ t,
+  has_type t .Nat -> value t -> nvalue t := by
+  intro t ty v
+  cases v with
+  | inl => cases ty <;> contradiction
+  | inr => assumption
+```
